lib/Lib.NTuple.fst
@@ -239,3 +239,13 @@ let tup4_lemma #a #l t =
   let (x0,(x1,(x2,x3))) = tup4 t in
   let t' : ntuple a 4 = (x0,(x1,(x2,x3))) in
   assert (t == t')
+
+#set-options "--max_fuel 9 --max_ifuel 8"
+let ntup8_lemma #a #l t = ()
+
+
+let tup8_lemma #a #l t =
+  assert (ntuple a l == ntuple a 8);
+  let (x0,(x1,(x2,(x3,(x4,(x5,(x6,x7))))))) = tup8 t in
+  let t' : ntuple a 8 = (x0,(x1,(x2,(x3,(x4,(x5,(x6,x7))))))) in
+  assert (t == t')
