code/sha2-vec/Hacl.Impl.SHA2.Core.fsti
@@ -1,0 +1,71 @@
+module Hacl.Impl.SHA2.Core
+open FStar.Mul
+module ST = FStar.HyperStack.ST
+open FStar.HyperStack
+open FStar.HyperStack.All
+open Lib.IntTypes
+open Lib.Sequence
+open Lib.Buffer
+open Lib.IntVector
+open Spec.Hash.Definitions
+open Hacl.Hash.Definitions
+module Spec = Hacl.Spec.SHA2
+
+val sha256: hash:lbuffer uint8 32ul -> len:size_t -> b:lbuffer uint8 len ->
+    Stack unit
+    (requires (fun h0 -> live h0 b /\ live h0 hash /\ disjoint hash b))
+    (ensures (fun h0 _ h1 -> modifies (loc hash) h0 h1 /\
+                           as_seq h1 hash == Spec.hash #SHA2_256 (v len) (as_seq h0 b)))
+
+
+val sha256_4: r0:lbuffer uint8 32ul ->
+              r1:lbuffer uint8 32ul ->
+              r2:lbuffer uint8 32ul ->
+              r3:lbuffer uint8 32ul ->
+              len:size_t ->
+              b0:lbuffer uint8 len ->
+              b1:lbuffer uint8 len ->
+              b2:lbuffer uint8 len ->
+              b3:lbuffer uint8 len ->
+    Stack unit
+    (requires (fun h0 -> live h0 b0 /\ live h0 b1 /\ live h0 b2 /\ live h0 b3 /\ 
+                       live h0 r0 /\ live h0 r1 /\ live h0 r2 /\ live h0 r3 /\
+                       disjoint r0 r1 /\ disjoint r0 r2 /\ disjoint r0 r3 /\
+                       disjoint r1 r2 /\ disjoint r1 r3 /\ disjoint r2 r3))
+    (ensures (fun h0 _ h1 -> modifies (loc r0 |+| loc r1 |+| loc r2 |+| loc r3) h0 h1 /\
+                           as_seq h1 r0 == Spec.hash #SHA2_256 (v len) (as_seq h0 b0) /\
+                           as_seq h1 r1 == Spec.hash #SHA2_256 (v len) (as_seq h0 b1) /\
+                           as_seq h1 r2 == Spec.hash #SHA2_256 (v len) (as_seq h0 b2) /\
+                           as_seq h1 r3 == Spec.hash #SHA2_256 (v len) (as_seq h0 b3)))
+
+
+
+val sha256_8: r0:lbuffer uint8 32ul ->
+              r1:lbuffer uint8 32ul ->
+              r2:lbuffer uint8 32ul ->
+              r3:lbuffer uint8 32ul ->
+              r4:lbuffer uint8 32ul ->
+              r5:lbuffer uint8 32ul ->
+              r6:lbuffer uint8 32ul ->
+              r7:lbuffer uint8 32ul ->
+              len:size_t ->
+              b0:lbuffer uint8 len ->
+              b1:lbuffer uint8 len ->
+              b2:lbuffer uint8 len ->
+              b3:lbuffer uint8 len ->
+              b4:lbuffer uint8 len ->
+              b5:lbuffer uint8 len ->
+              b6:lbuffer uint8 len ->
+              b7:lbuffer uint8 len ->
+    Stack unit
+    (requires (fun h0 -> live h0 b0 /\ live h0 b1 /\ live h0 b2 /\ live h0 b3 /\ live h0 b4 /\ live h0 b5 /\ live h0 b6 /\ live h0 b7 /\  
+                       live h0 r0 /\ live h0 r1 /\ live h0 r2 /\ live h0 r3 /\ live h0 r4 /\ live h0 r5 /\ live h0 r6 /\ live h0 r7 /\
+                       disjoint r0 r1 /\ disjoint r0 r2 /\ disjoint r0 r3 /\
+                       disjoint r1 r2 /\ disjoint r1 r3 /\ disjoint r2 r3))
+    (ensures (fun h0 _ h1 -> modifies (loc r0 |+| loc r1 |+| loc r2 |+| loc r3) h0 h1 /\
+                           as_seq h1 r0 == Spec.hash #SHA2_256 (v len) (as_seq h0 b0) /\
+                           as_seq h1 r1 == Spec.hash #SHA2_256 (v len) (as_seq h0 b1) /\
+                           as_seq h1 r2 == Spec.hash #SHA2_256 (v len) (as_seq h0 b2) /\
+                           as_seq h1 r3 == Spec.hash #SHA2_256 (v len) (as_seq h0 b3)))
+
+
