code/sha2-vec/Hacl.Spec.SHA2.Equiv.fst
@@ -784,3 +784,4 @@ val hash_lemma:
 
 let hash_lemma #a #m len b =
   Classical.forall_intro (hash_lemma_l #a #m len b)
+  
